06TailCall/TailCallOptimization.thy
@@ -9,21 +9,24 @@ fun tco_r :: "tree_code list \<Rightarrow> tco_return" where
     | _ \<Rightarrow> tco_r cd)"
 | "tco_r (op # cd) = tco_r cd"
 
-fun tco :: "tree_code list \<Rightarrow> tco_code list" where
-  "tco [] = []"
-| "tco (TLookup x # cd) = TCOLookup x # tco cd"
-| "tco (TPushCon k # cd) = TCOPushCon k # tco cd"
-| "tco (TPushLam cd' # cd) = TCOPushLam (tco cd') (tco_r cd') # tco cd"
-| "tco (TApply # cd) = (case cd of 
+fun tco_cd :: "tree_code list \<Rightarrow> tco_code list" where
+  "tco_cd [] = []"
+| "tco_cd (TLookup x # cd) = TCOLookup x # tco_cd cd"
+| "tco_cd (TPushCon k # cd) = TCOPushCon k # tco_cd cd"
+| "tco_cd (TPushLam cd' # cd) = TCOPushLam (tco_cd cd') (tco_r cd') # tco_cd cd"
+| "tco_cd (TApply # cd) = (case cd of 
       [] \<Rightarrow> []
-    | _ \<Rightarrow> TCOApply # tco cd)"
+    | _ \<Rightarrow> TCOApply # tco_cd cd)"
+
+definition tco :: "tree_code list \<Rightarrow> tco_code list \<times> tco_return" where
+  "tco cd = (tco_cd cd, tco_r cd)"
 
 primrec tco_val :: "tclosure \<Rightarrow> tco_closure" where
   "tco_val (TConst k) = TCOConst k"
-| "tco_val (TLam vs cd) = TCOLam (map tco_val vs) (tco cd) (tco_r cd)"
+| "tco_val (TLam vs cd) = TCOLam (map tco_val vs) (tco_cd cd) (tco_r cd)"
 
 fun tco_stack_frame :: "tree_stack_frame \<Rightarrow> tco_stack_frame" where
-  "tco_stack_frame (vs, cd) = (map tco_val vs, tco cd, tco_r cd)"
+  "tco_stack_frame (vs, cd) = (map tco_val vs, tco_cd cd, tco_r cd)"
 
 fun not_dead_frame :: "tco_stack_frame \<Rightarrow> bool" where
   "not_dead_frame (vs, cd, r) = (cd \<noteq> [] \<or> r \<noteq> TCOReturn)"
@@ -38,7 +41,7 @@ primrec tco_state :: "tree_code_state \<Rightarrow> tco_code_state" where
   "tco_state (TS vs sfs) = TCOS (map tco_val vs) (tco_stack sfs)"
 
 lemma [dest]: "(env, cd, r) # sfs = tco_stack sfs' \<Longrightarrow> \<exists>dsfs env' cd' sfs''. 
-  sfs' = dsfs @ (env', cd') # sfs'' \<and> env = map tco_val env' \<and> cd = tco cd' \<and> r = tco_r cd' \<and> 
+  sfs' = dsfs @ (env', cd') # sfs'' \<and> env = map tco_val env' \<and> cd = tco_cd cd' \<and> r = tco_r cd' \<and> 
     list_all dead_frame dsfs \<and> sfs = tco_stack sfs''"
 proof (induction sfs')
   case (Cons sf sfs')
@@ -46,11 +49,10 @@ proof (induction sfs')
   proof (induction sf)
     case (Pair env' cd')
     thus ?case
-    proof (induction cd' rule: tco.induct)
-
+    proof (induction cd' rule: tco_cd.induct)
       case 1
       then obtain dsfs env'' cd' sfs'' where X: "sfs' = dsfs @ (env'', cd') # sfs'' \<and> 
-        env = map tco_val env'' \<and> cd = tco cd' \<and> r = tco_r cd' \<and> list_all dead_frame dsfs \<and> 
+        env = map tco_val env'' \<and> cd = tco_cd cd' \<and> r = tco_r cd' \<and> list_all dead_frame dsfs \<and> 
           sfs = tco_stack sfs''" by auto
       hence "\<exists>dsfsx. (env', []) # dsfs @ (env'', cd') # sfs'' = dsfsx @ (env'', cd') # sfs'' \<and> 
           list_all dead_frame dsfsx \<and> sfs = tco_stack sfs''" by simp
@@ -60,17 +62,17 @@ proof (induction sfs')
       with X show ?case by fastforce
     next
       case (2 x cd')
-      hence "env = map tco_val env' \<and> cd = TCOLookup x # tco cd' \<and> r = tco_r cd' \<and> 
+      hence "env = map tco_val env' \<and> cd = TCOLookup x # tco_cd cd' \<and> r = tco_r cd' \<and> 
         sfs = tco_stack sfs'" by simp
       thus ?case by fastforce
     next
       case (3 k cd')
-      hence "env = map tco_val env' \<and> cd = TCOPushCon k # tco cd' \<and> r = tco_r cd' \<and> 
+      hence "env = map tco_val env' \<and> cd = TCOPushCon k # tco_cd cd' \<and> r = tco_r cd' \<and> 
         sfs = tco_stack sfs'" by simp
       thus ?case by fastforce
     next
       case (4 cd\<^sub>l cd')
-      hence "env = map tco_val env' \<and> cd = TCOPushLam (tco cd\<^sub>l) (tco_r cd\<^sub>l) # tco cd' \<and> 
+      hence "env = map tco_val env' \<and> cd = TCOPushLam (tco_cd cd\<^sub>l) (tco_r cd\<^sub>l) # tco_cd cd' \<and> 
         r = tco_r cd' \<and> sfs = tco_stack sfs'" by simp
       thus ?case by fastforce
     next
@@ -83,7 +85,7 @@ proof (induction sfs')
         ultimately show ?thesis by fastforce
       next
         case (Cons op cd'')
-        moreover with 5 have "env = map tco_val env' \<and> cd = TCOApply # tco (op # cd'') \<and> 
+        moreover with 5 have "env = map tco_val env' \<and> cd = TCOApply # tco_cd (op # cd'') \<and> 
           r = tco_r (op # cd'') \<and> sfs = tco_stack sfs'" by simp
         ultimately show ?thesis by fastforce
       qed
@@ -93,11 +95,11 @@ qed simp_all
 
 lemma [dest]: "TCOS vs ((env, cd, r) # sfs) = tco_state \<Sigma> \<Longrightarrow> \<exists>dsfs vs' env' cd' sfs'. 
   \<Sigma> = TS vs' (dsfs @ (env', cd') # sfs') \<and> vs = map tco_val vs' \<and> env = map tco_val env' \<and> 
-    cd = tco cd' \<and> r = tco_r cd' \<and> list_all dead_frame dsfs \<and> sfs = tco_stack sfs'"
+    cd = tco_cd cd' \<and> r = tco_r cd' \<and> list_all dead_frame dsfs \<and> sfs = tco_stack sfs'"
   by (induction \<Sigma>) auto
 
-lemma [dest]: "TCOLookup x # cd = tco cd' \<Longrightarrow> \<exists>cd''. cd' = TLookup x # cd'' \<and> cd = tco cd''"
-  by (induction cd' rule: tco.induct) (simp_all split: list.splits)
+lemma [dest]: "TCOLookup x # cd = tco_cd cd' \<Longrightarrow> \<exists>cd''. cd' = TLookup x # cd'' \<and> cd = tco_cd cd''"
+  by (induction cd' rule: tco_cd.induct) (simp_all split: list.splits)
 
 lemma [simp]: "list_all dead_frame dsfs \<Longrightarrow> iter (\<leadsto>\<^sub>t) (TS vs (dsfs @ sfs)) (TS vs sfs)"
 proof (induction dsfs)
@@ -108,16 +110,16 @@ proof (induction dsfs)
 qed simp_all
 
 lemma [simp]: "\<exists>\<Sigma>\<^sub>t \<Sigma>. iter (\<leadsto>\<^sub>t) (TS vs ((env, cd) # sfs)) \<Sigma>\<^sub>t \<and> 
-  iter (\<leadsto>\<^sub>t\<^sub>c\<^sub>o) (TCOS (map tco_val vs) ((map tco_val env, tco cd, tco_r cd) # tco_stack sfs)) \<Sigma> \<and> 
+  iter (\<leadsto>\<^sub>t\<^sub>c\<^sub>o) (TCOS (map tco_val vs) ((map tco_val env, tco_cd cd, tco_r cd) # tco_stack sfs)) \<Sigma> \<and> 
     \<Sigma> = tco_state \<Sigma>\<^sub>t" 
-proof (induction cd rule: tco.induct)
+proof (induction cd rule: tco_cd.induct)
   case 1
   have "TS vs ((env, []) # sfs) \<leadsto>\<^sub>t TS vs sfs" by simp
   hence X: "iter (\<leadsto>\<^sub>t) (TS vs ((env, []) # sfs)) (TS vs sfs)" by (metis iter_one)
-  have "TCOS (map tco_val vs) ((map tco_val env, tco [], tco_r []) # tco_stack sfs) \<leadsto>\<^sub>t\<^sub>c\<^sub>o
+  have "TCOS (map tco_val vs) ((map tco_val env, tco_cd [], tco_r []) # tco_stack sfs) \<leadsto>\<^sub>t\<^sub>c\<^sub>o
     TCOS (map tco_val vs) (tco_stack sfs)" by simp
   hence Y: "iter (\<leadsto>\<^sub>t\<^sub>c\<^sub>o) 
-    (TCOS (map tco_val vs) ((map tco_val env, tco [], tco_r []) # tco_stack sfs)) 
+    (TCOS (map tco_val vs) ((map tco_val env, tco_cd [], tco_r []) # tco_stack sfs)) 
       (TCOS (map tco_val vs) (tco_stack sfs))" by (metis iter_one)
   have "TCOS (map tco_val vs) (tco_stack sfs) = tco_state (TS vs sfs)" by simp
   with X Y show ?case by blast
@@ -127,7 +129,7 @@ next
 
   have X: "iter (\<leadsto>\<^sub>t) (TS vs ((env, TLookup x # cd) # sfs)) \<Sigma>\<^sub>t" by simp
   have Y: "iter (\<leadsto>\<^sub>t\<^sub>c\<^sub>o) (TCOS (map tco_val vs) 
-    ((map tco_val env, tco (TLookup x # cd), tco_r (TLookup x # cd)) # tco_stack sfs)) \<Sigma>" by simp
+    ((map tco_val env, tco_cd (TLookup x # cd), tco_r (TLookup x # cd)) # tco_stack sfs)) \<Sigma>" by simp
   have "\<Sigma> = tco_state \<Sigma>\<^sub>t" by simp
   with X Y show ?case by blast
 next
@@ -146,9 +148,9 @@ theorem completetco [simp]: "tco_state \<Sigma>\<^sub>t \<leadsto>\<^sub>t\<^sub
 proof (induction "tco_state \<Sigma>\<^sub>t" \<Sigma>' rule: evaltco.induct)
   case (evtco_lookup env x v vs cd r sfs)
   then obtain dsfs vs' env' cd' sfs' where S: "\<Sigma>\<^sub>t = TS vs' (dsfs @ (env', cd') # sfs') \<and> 
-    vs = map tco_val vs' \<and> env = map tco_val env' \<and> TCOLookup x # cd = tco cd' \<and> r = tco_r cd' \<and> 
+    vs = map tco_val vs' \<and> env = map tco_val env' \<and> TCOLookup x # cd = tco_cd cd' \<and> r = tco_r cd' \<and> 
       list_all dead_frame dsfs \<and> sfs = tco_stack sfs'" by blast
-  then obtain cd'' where C: "cd' = TLookup x # cd'' \<and> cd = tco cd''" by blast
+  then obtain cd'' where C: "cd' = TLookup x # cd'' \<and> cd = tco_cd cd''" by blast
   from evtco_lookup S obtain v' where V: "lookup env' x = Some v' \<and> v = tco_val v'" by auto
   hence "TS vs' ((env', TLookup x # cd'') # sfs') \<leadsto>\<^sub>t TS (v' # vs') ((env', cd'') # sfs')" by simp
   moreover from S have "iter (\<leadsto>\<^sub>t) (TS vs' (dsfs @ (env', TLookup x # cd'') # sfs')) 
@@ -177,11 +179,11 @@ next
   then show ?case by simp
 qed
 
-lemma [simp]: "tco (op # cd) = [] \<Longrightarrow> tco_r (op # cd) = TCOJump"
+lemma [simp]: "tco_cd (op # cd) = [] \<Longrightarrow> tco_r (op # cd) = TCOJump"
   by (induction op) (simp_all split: list.splits)
 
-lemma tco_never_dead [simp]: "not_dead_frame (vs, tco (op # cd), tco_r (op # cd))"
-  by (induction cd rule: tco.induct) (simp_all split: list.splits)
+lemma tco_never_dead [simp]: "not_dead_frame (vs, tco_cd (op # cd), tco_r (op # cd))"
+  by (induction cd rule: tco_cd.induct) (simp_all split: list.splits)
 
 theorem correcttco [simp]: "\<Sigma> \<leadsto>\<^sub>t \<Sigma>' \<Longrightarrow> iter (\<leadsto>\<^sub>t\<^sub>c\<^sub>o) (tco_state \<Sigma>) (tco_state \<Sigma>')"
 proof (induction \<Sigma> \<Sigma>' rule: evalt.induct)
@@ -228,9 +230,9 @@ next
   proof (cases cd)
     case Nil
     have "tco_state (TS vs ((env, [TPushLam cd']) # sfs)) \<leadsto>\<^sub>t\<^sub>c\<^sub>o
-      TCOS (TCOLam (map tco_val env) (tco cd') (tco_r cd') # map tco_val vs) 
+      TCOS (TCOLam (map tco_val env) (tco_cd cd') (tco_r cd') # map tco_val vs) 
         ((map tco_val env, [], TCOReturn) # tco_stack sfs)" by simp
-    moreover have "TCOS (TCOLam (map tco_val env) (tco cd') (tco_r cd') # map tco_val vs) 
+    moreover have "TCOS (TCOLam (map tco_val env) (tco_cd cd') (tco_r cd') # map tco_val vs) 
       ((map tco_val env, [], TCOReturn) # tco_stack sfs) \<leadsto>\<^sub>t\<^sub>c\<^sub>o
         tco_state (TS (TLam env cd' # vs) ((env, []) # sfs))" by simp
     ultimately have "iter (\<leadsto>\<^sub>t\<^sub>c\<^sub>o) (tco_state (TS vs ((env, [TPushLam cd']) # sfs)))
@@ -243,28 +245,28 @@ next
     ultimately show ?thesis by (metis iter_one)
   qed
 next
-  case (evt_apply v env cd' vs cd sfs)
+  case (evt_apply v env' cd' vs env cd sfs)
   thus ?case 
   proof (cases cd)
     case Nil note CD = Nil
     thus ?thesis
     proof (cases cd')
       case Nil
-      have "TCOS (map tco_val vs) ((tco_val v # map tco_val env, [], TCOReturn) # tco_stack sfs) 
-        \<leadsto>\<^sub>t\<^sub>c\<^sub>o tco_state (TS vs ((v # env, []) # (env, []) # sfs))" by simp
+      have "TCOS (map tco_val vs) ((tco_val v # map tco_val env', [], TCOReturn) # tco_stack sfs) 
+        \<leadsto>\<^sub>t\<^sub>c\<^sub>o tco_state (TS vs ((v # env', []) # (env, []) # sfs))" by simp
       hence "iter (\<leadsto>\<^sub>t\<^sub>c\<^sub>o) (TCOS (map tco_val vs) 
-        ((tco_val v # map tco_val env, [], TCOReturn) # tco_stack sfs))
-          (tco_state (TS vs ((v # env, []) # (env, []) # sfs)))" by (metis iter_one)
-      moreover have "tco_state (TS (v # TLam env [] # vs) ((env, [TApply]) # sfs)) \<leadsto>\<^sub>t\<^sub>c\<^sub>o
-        TCOS (map tco_val vs) ((tco_val v # map tco_val env, [], TCOReturn) # tco_stack sfs)" 
+        ((tco_val v # map tco_val env', [], TCOReturn) # tco_stack sfs))
+          (tco_state (TS vs ((v # env', []) # (env, []) # sfs)))" by (metis iter_one)
+      moreover have "tco_state (TS (v # TLam env' [] # vs) ((env, [TApply]) # sfs)) \<leadsto>\<^sub>t\<^sub>c\<^sub>o
+        TCOS (map tco_val vs) ((tco_val v # map tco_val env', [], TCOReturn) # tco_stack sfs)" 
           by simp
-      ultimately have "iter (\<leadsto>\<^sub>t\<^sub>c\<^sub>o) (tco_state (TS (v # TLam env [] # vs) ((env, [TApply]) # sfs)))
-        (tco_state (TS vs ((v # env, []) # (env, []) # sfs)))" using iter_step by fast
-      with CD Nil show ?thesis by simpx
+      ultimately have "iter (\<leadsto>\<^sub>t\<^sub>c\<^sub>o) (tco_state (TS (v # TLam env' [] # vs) ((env, [TApply]) # sfs)))
+        (tco_state (TS vs ((v # env', []) # (env, []) # sfs)))" using iter_step by fast
+      with CD Nil show ?thesis by simp
     next
-      case (Cons op' cd')
-      have "tco_state (TS (v # TLam env (op' # cd') # vs) ((env, [TApply]) # sfs)) \<leadsto>\<^sub>t\<^sub>c\<^sub>o
-        tco_state (TS vs ((v # env, op' # cd') # (env, []) # sfs))" by simp
+      case (Cons op' cd'')
+      have "tco_state (TS (v # TLam env' (op' # cd'') # vs) ((env, [TApply]) # sfs)) \<leadsto>\<^sub>t\<^sub>c\<^sub>o
+        tco_state (TS vs ((v # env', op' # cd'') # (env, []) # sfs))" by simp
       with Nil Cons show ?thesis by (metis iter_one)
     qed
   next
@@ -272,25 +274,25 @@ next
     thus ?thesis
     proof (cases cd')
       case Nil
-      have "TCOS (map tco_val vs) ((tco_val v # map tco_val env, [], TCOReturn) # 
-        (map tco_val env, tco (op # cd), tco_r (op # cd)) # tco_stack sfs) \<leadsto>\<^sub>t\<^sub>c\<^sub>o
-          tco_state (TS vs ((v # env, []) # (env, op # cd) # sfs))" by simp
-      hence "iter (\<leadsto>\<^sub>t\<^sub>c\<^sub>o) (TCOS (map tco_val vs) ((tco_val v # map tco_val env, [], TCOReturn) # 
-        (map tco_val env, tco (op # cd), tco_r (op # cd)) # tco_stack sfs)) 
-          (tco_state (TS vs ((v # env, []) # (env, op # cd) # sfs)))" by (metis iter_one)
-      moreover have "tco_state (TS (v # TLam env [] # vs) ((env, TApply # op # cd) # sfs)) \<leadsto>\<^sub>t\<^sub>c\<^sub>o
-        TCOS (map tco_val vs) ((tco_val v # map tco_val env, [], TCOReturn) # 
-          (map tco_val env, tco (op # cd), tco_r (op # cd)) # tco_stack sfs)" by simp
-      ultimately have "iter (\<leadsto>\<^sub>t\<^sub>c\<^sub>o) (tco_state (TS (v # TLam env [] # vs) 
+      have "TCOS (map tco_val vs) ((tco_val v # map tco_val env', [], TCOReturn) # 
+        (map tco_val env, tco_cd (op # cd), tco_r (op # cd)) # tco_stack sfs) \<leadsto>\<^sub>t\<^sub>c\<^sub>o
+          tco_state (TS vs ((v # env', []) # (env, op # cd) # sfs))" by simp
+      hence "iter (\<leadsto>\<^sub>t\<^sub>c\<^sub>o) (TCOS (map tco_val vs) ((tco_val v # map tco_val env', [], TCOReturn) # 
+        (map tco_val env, tco_cd (op # cd), tco_r (op # cd)) # tco_stack sfs)) 
+          (tco_state (TS vs ((v # env', []) # (env, op # cd) # sfs)))" by (metis iter_one)
+      moreover have "tco_state (TS (v # TLam env' [] # vs) ((env, TApply # op # cd) # sfs)) \<leadsto>\<^sub>t\<^sub>c\<^sub>o
+        TCOS (map tco_val vs) ((tco_val v # map tco_val env', [], TCOReturn) # 
+          (map tco_val env, tco_cd (op # cd), tco_r (op # cd)) # tco_stack sfs)" by simp
+      ultimately have "iter (\<leadsto>\<^sub>t\<^sub>c\<^sub>o) (tco_state (TS (v # TLam env' [] # vs) 
         ((env, TApply # op # cd) # sfs)))
-          (tco_state (TS vs ((v # env, []) # (env, op # cd) # sfs)))" 
+          (tco_state (TS vs ((v # env', []) # (env, op # cd) # sfs)))" 
         using iter_step by fast
-      with Cons Nil show ?thesis by simpx
+      with Cons Nil show ?thesis by simp
     next
       case (Cons op' cd')
-      from evt_lookup have "tco_state (TS (v # TLam env (op' # cd') # vs) 
+      from evt_lookup have "tco_state (TS (v # TLam env' (op' # cd') # vs) 
         ((env, TApply # op # cd) # sfs)) \<leadsto>\<^sub>t\<^sub>c\<^sub>o
-          tco_state (TS vs ((v # env, (op' # cd')) # (env, op # cd) # sfs))" by simp
+          tco_state (TS vs ((v # env', (op' # cd')) # (env, op # cd) # sfs))" by simp
       with CD Cons show ?thesis by (metis iter_one)
     qed
   qed
