07FlatCode/CodeFlattening.thy
@@ -12,18 +12,18 @@ fun flatten_code' :: "nat \<Rightarrow> tco_code list \<Rightarrow> tco_return \
     in clo @ flatten_code' (lib + length clo) cd r (BPushLam (lib + length clo) # acc))"
 | "flatten_code' lib (TCOApply # cd) r acc = flatten_code' lib cd r (BApply # acc)"
 
-definition flatten_code :: "tco_code list \<Rightarrow> byte_code list" where
-  "flatten_code cd = flatten_code' 0 cd TCOReturn []"
+primrec flatten_code :: "tco_code list \<times> tco_return \<Rightarrow> byte_code list" where
+  "flatten_code (cd, r) = flatten_code' 0 cd r []"
 
 fun unflatten_return :: "byte_code list \<Rightarrow> nat \<Rightarrow> tco_return" where
   "unflatten_return cd 0 = undefined"
 | "unflatten_return cd (Suc pc) = (case cd ! pc of
-       BReturn \<Rightarrow> TCOReturn
+      BReturn \<Rightarrow> TCOReturn
     | BJump \<Rightarrow> TCOJump
     | op \<Rightarrow> unflatten_return cd pc)"
 
 fun unflatten_code :: "byte_code list \<Rightarrow> nat \<Rightarrow> tco_code list" where
-  "unflatten_code cd 0 = undefined"
+  "unflatten_code cd 0 = []"
 | "unflatten_code cd (Suc pc) = (case cd ! pc of
       BLookup x \<Rightarrow> TCOLookup x # unflatten_code cd pc
     | BPushCon k \<Rightarrow>  TCOPushCon k # unflatten_code cd pc
@@ -43,8 +43,11 @@ primrec unflatten_closure :: "byte_code list \<Rightarrow> bclosure \<Rightarrow
 abbreviation ufcs :: "byte_code list \<Rightarrow> bclosure list \<Rightarrow> tco_closure list" where
   "ufcs cd vs \<equiv> map (unflatten_closure cd) vs"
 
+primrec ufsf :: "byte_code list \<Rightarrow> (bclosure list \<times> nat) \<Rightarrow> tco_stack_frame" where
+  "ufsf cd (vs, pc) = (ufcs cd vs, unflatten_code cd pc, unflatten_return cd pc)"
+
 abbreviation ufsfs :: "byte_code list \<Rightarrow> (bclosure list \<times> nat) list \<Rightarrow> tco_stack_frame list" where
-  "ufsfs cd pcs \<equiv> map (\<lambda>(vs, pc). (ufcs cd vs, unflatten_code cd pc, unflatten_return cd pc)) pcs"
+  "ufsfs cd pcs \<equiv> map (ufsf cd) pcs"
 
 primrec unflatten_state :: "byte_code_state \<Rightarrow> tco_code_state" where
   "unflatten_state (BS vs sfs cd) = TCOS (ufcs cd vs) (ufsfs cd sfs)"
@@ -53,9 +56,9 @@ primrec code_size :: "tco_code \<Rightarrow> nat"
     and code_list_size :: "tco_code list \<Rightarrow> nat" where
   "code_size (TCOLookup x) = 1"
 | "code_size (TCOPushCon k) = 1"
-| "code_size (TCOPushLam cd r) = Suc (Suc (code_list_size cd))"
+| "code_size (TCOPushLam cd r) = Suc (code_list_size cd)"
 | "code_size TCOApply = 1"
-| "code_list_size [] = 0"
+| "code_list_size [] = 1"
 | "code_list_size (c # cd) = code_size c + code_list_size cd"
 
 fun ordered :: "byte_code \<Rightarrow> nat \<Rightarrow> bool" where
@@ -77,17 +80,20 @@ primrec return_terminated :: "byte_code list \<Rightarrow> bool" where
   "return_terminated [] = False"
 | "return_terminated (op # cd) = (op = BReturn \<or> op = BJump)"
 
+fun orderly_stack :: "(bclosure list \<times> nat) list \<Rightarrow> nat \<Rightarrow> bool" where
+  "orderly_stack [] cd = True"
+| "orderly_stack ((env, 0) # sfs) cd = False"
+| "orderly_stack ((env, Suc pc) # sfs) cd = 
+    (pc < cd \<and> ordered_closures env cd \<and> orderly_stack sfs cd)"
+
 primrec orderly_state :: "byte_code_state \<Rightarrow> bool" where
   "orderly_state (BS vs sfs cd) = (orderly cd 0 \<and> return_terminated cd \<and> 
-    (\<forall>(env, pc) \<in> set sfs. 0 < pc \<and> pc \<le> length cd \<and> ordered_closures env (length cd)) \<and> 
-      (ordered_closures vs (length cd)))"
+    orderly_stack sfs (length cd) \<and> ordered_closures vs (length cd))"
 
-(*
+lemma flatten_length [simp]: "length (flatten_code' lib cd r acc) = code_list_size cd + length acc"
+  by (induction lib cd r acc rule: flatten_code'.induct) simp_all
 
-lemma flatten_length [simp]: "length (flatten_code' lib cd acc) = code_list_size cd + length acc"
-  by (induction lib cd acc rule: flatten_code'.induct) simp_all
-
-lemma [simp]: "length (flatten_code cd) = code_list_size cd"
+lemma [simp]: "length (flatten_code (cd, r)) = code_list_size cd"
   by (simp add: flatten_code_def)
 
 lemma [simp]: "Suc 0 \<le> code_list_size cd"
@@ -96,24 +102,20 @@ lemma [simp]: "Suc 0 \<le> code_list_size cd"
 lemma [simp]: "0 < code_list_size cd"
   by (induction cd) simp_all
 
-lemma [simp]: "flatten_code' cd lib acc \<noteq> []"
-  by (induction cd lib acc rule: flatten_code'.induct) simp_all
+lemma [simp]: "flatten_code' lib cd r acc \<noteq> []"
+  by (induction lib cd r acc rule: flatten_code'.induct) simp_all
 
-lemma [simp]: "flatten_code cd \<noteq> []"
+lemma [simp]: "flatten_code (cd, r) \<noteq> []"
   by (simp add: flatten_code_def)
 
-lemma [simp]: "flatten_code' cd lib acc ! 0 = BReturn_Old"
-proof (induction cd lib acc rule: flatten_code'.induct)
-  case (4 lib cd' cd acc)
-  moreover have "length (flatten_code' lib cd' []) > 0" by simp
-  ultimately have "(flatten_code' lib cd' [] @ 
-    flatten_code' (lib + code_list_size cd') cd (BPushLam (lib + code_list_size cd') # acc)) ! 0 =
-      BReturn_Old" by (metis nth_append)
-  thus ?case by simp
-qed simp_all
+lemma [simp]: "cd \<noteq> [] \<Longrightarrow> return_terminated (cd @ cd') = return_terminated cd"
+  by (induction cd) simp_all
 
-lemma [simp]: "flatten_code cd ! 0 = BReturn_Old"
-  by (simp add: flatten_code_def)
+lemma [simp]: "return_terminated (flatten_code' lib cd r acc)"
+  by (induction lib cd r acc rule: flatten_code'.induct) simp_all
+
+lemma [simp]: "return_terminated (flatten_code cdr)"
+  by (cases cdr) (simp add: flatten_code_def)
 
 lemma [simp]: "ordered op x \<Longrightarrow> ordered op (Suc x)"
   by (induction op) simp_all
@@ -132,11 +134,17 @@ lemma [simp]: "orderly (cd @ cd') n = (orderly cd n \<and> orderly cd' (length c
   by (induction cd arbitrary: n) simp_all
 
 lemma [simp]: "\<forall>x < length acc. ordered (acc ! x) (x + n) \<Longrightarrow> lib \<le> n \<Longrightarrow> 
-    orderly (flatten_code' lib cd acc) n"
-  by (induction lib cd acc arbitrary: n rule: flatten_code'.induct) simp_all
+    orderly (flatten_code' lib cd r acc) n"
+  by (induction lib cd r acc arbitrary: n rule: flatten_code'.induct) simp_all
 
-lemma [simp]: "orderly (flatten_code cd) 0"
-  by (simp add: flatten_code_def)
+lemma [simp]: "orderly (flatten_code cdr) 0"
+  by (cases cdr) (simp add: flatten_code_def)
+
+lemma [simp]: "x > 0 \<Longrightarrow> orderly_stack [([], x)] x"
+  by (cases x) simp_all
+
+lemma [simp]: "orderly_stack [([], length (flatten_code cdr))] (length (flatten_code cdr))"
+  by (cases cdr) simp_all
 
 lemma [simp]: "lookup vs x = Some v \<Longrightarrow> ordered_closures vs n \<Longrightarrow> ordered_closure v n"
   by (induction vs x rule: lookup.induct) simp_all
@@ -149,59 +157,58 @@ lemma [simp]: "cd ! x = BPushLam pc \<Longrightarrow> orderly cd 0 \<Longrightar
   using pushlam_ordered by fastforce
 
 lemma index_into_append [simp]: 
-  "(flatten_code' lib cd [] @ cd') ! (code_list_size cd + n) = cd' ! n"
+  "(flatten_code' lib cd r [] @ cd') ! (code_list_size cd + n) = cd' ! n"
     by (metis add.right_neutral flatten_length list.size(3) nth_append_length_plus)
 
-lemma index_into_flatten [simp]: "flatten_code' lib cd acc ! (n + code_list_size cd) = acc ! n"
-proof (induction lib cd acc arbitrary: n rule: flatten_code'.induct)
-  case (2 lib x cd acc)
-  hence "flatten_code' lib cd (BLookup x # acc) ! (Suc n + code_list_size cd) = 
+lemma index_into_flatten [simp]: "flatten_code' lib cd r acc ! (n + code_list_size cd) = acc ! n"
+proof (induction lib cd r acc arbitrary: n rule: flatten_code'.induct)
+  case (3 lib x cd r acc)
+  hence "flatten_code' lib cd r (BLookup x # acc) ! (Suc n + code_list_size cd) = 
     (BLookup x # acc) ! Suc n" by blast
-  then show ?case by simp
+  thus ?case by simp
 next
-  case (3 lib k cd acc)
-  hence "flatten_code' lib cd (BPushCon k # acc) ! (Suc n + code_list_size cd) = 
+  case (4 lib k cd r acc)
+  hence "flatten_code' lib cd r (BPushCon k # acc) ! (Suc n + code_list_size cd) = 
     (BPushCon k # acc) ! Suc n" by blast
-  then show ?case by simp
+  thus ?case by simp
 next
-  case (4 lib cd' cd acc)
-  hence "flatten_code' (lib + length (flatten_code' lib cd' [])) cd 
-    (BPushLam (lib + length (flatten_code' lib cd' [])) # acc) ! (Suc n + code_list_size cd) = 
-      (BPushLam (lib + length (flatten_code' lib cd' [])) # acc) ! Suc n" by blast
-  hence "flatten_code' (lib + code_list_size cd') cd 
-    (BPushLam (lib + code_list_size cd') # acc) ! Suc (n + code_list_size cd) = acc ! n" by simp
-  hence "(flatten_code' lib cd' [] @ flatten_code' (lib + code_list_size cd') cd 
+  case (5 lib cd' r' cd r acc)
+  let ?cd' = "flatten_code' lib cd' r' []"
+  from 5 have "flatten_code' (lib + length ?cd') cd r (BPushLam (lib + length ?cd') # acc) ! 
+    (Suc n + code_list_size cd) = (BPushLam (lib + length ?cd') # acc) ! Suc n" by blast
+  hence "flatten_code' (lib + code_list_size cd') cd r (BPushLam (lib + code_list_size cd') # acc) ! 
+    Suc (n + code_list_size cd) = acc ! n" by simp
+  hence "(?cd' @ flatten_code' (lib + code_list_size cd') cd r 
     (BPushLam (lib + code_list_size cd') # acc)) !
       (code_list_size cd' + Suc (n + code_list_size cd)) = acc ! n" by (metis index_into_append)
   moreover have "code_list_size cd' + Suc (n + code_list_size cd) = 
     Suc (n + (code_list_size cd' + code_list_size cd))" by simp
-  ultimately have "(flatten_code' lib cd' [] @ flatten_code' (lib + code_list_size cd') cd 
+  ultimately have "(?cd' @ flatten_code' (lib + code_list_size cd') cd r 
     (BPushLam (lib + code_list_size cd') # acc)) !
       Suc (n + (code_list_size cd' + code_list_size cd)) = acc ! n" by metis
   thus ?case by simp
 next
-  case (5 lib cd acc)
-  hence "flatten_code' lib cd (BApply # acc) ! (Suc n + code_list_size cd) = 
+  case (6 lib cd r acc)
+  hence "flatten_code' lib cd r (BApply # acc) ! (Suc n + code_list_size cd) = 
     (BApply # acc) ! Suc n" by blast
-  then show ?case by simp
-next
-  case (6 lib cd acc)
-  hence "flatten_code' lib cd (BReturn # acc) ! (Suc n + code_list_size cd) = 
-    (BReturn # acc) ! Suc n" by blast
-  then show ?case by simp
-next
-  case (7 lib cd acc)
-  hence "flatten_code' lib cd (BJump # acc) ! (Suc n + code_list_size cd) = 
-    (BJump # acc) ! Suc n" by blast
-  then show ?case by simp
+  thus ?case by simp
 qed simp_all
 
-lemma [simp]: "flatten_code' lib cd (op # acc) ! code_list_size cd = op"
+lemma [simp]: "flatten_code' lib cd r (op # acc) ! code_list_size cd = op"
 proof -
-  have "flatten_code' lib cd (op # acc) ! (0 + code_list_size cd) = (op # acc) ! 0" 
+  have "flatten_code' lib cd r (op # acc) ! (0 + code_list_size cd) = (op # acc) ! 0" 
     by (metis index_into_flatten)
   thus ?thesis by simp
 qed
+
+lemma unflatten_r_front [simp]: "pc \<le> length cd \<Longrightarrow> 
+  unflatten_return (cd @ cd') pc = unflatten_return cd pc"
+proof (induction cd pc rule: unflatten_return.induct)
+  case (2 cd pc)
+  hence "pc < length cd" by simp
+  hence "(cd @ cd') ! pc = cd ! pc" by (metis nth_append)
+  with 2 show ?case by (cases "cd ! pc") simp_all
+qed simp_all
 
 lemma unflatten_front [simp]: "pc \<le> length cd \<Longrightarrow> 
   unflatten_code (cd @ cd') pc = unflatten_code cd pc"
@@ -212,401 +219,246 @@ proof (induction cd pc rule: unflatten_code.induct)
   with 2 show ?case by (cases "cd ! pc") simp_all
 qed simp_all
 
-lemma unflatten_flatten [simp]: "return_terminated cd \<Longrightarrow> 
-  unflatten_code (lib @ flatten_code' (length lib) cd acc) (length lib + code_list_size cd) = cd"
-proof (induction "length lib" cd acc arbitrary: lib rule: flatten_code'.induct)
-  case (4 cd' cd acc)
+lemma unflatten_flatten_r [simp]: "unflatten_return (lib @ flatten_code' (length lib) cd r acc) 
+  (length lib + code_list_size cd) = r"
+proof (induction "length lib" cd r acc arbitrary: lib rule: flatten_code'.induct)
+  case (5 cd' r' cd r acc)
   let ?pc = "length lib + code_list_size cd'"
-  let ?code' = "lib @ flatten_code' (length lib) cd' []"
-  let ?code = "?code' @ flatten_code' ?pc cd (BPushLam ?pc # acc)"
-  have Y: "length lib + length (flatten_code' (length lib) cd' []) = length ?code'" by simp
-  from 4 have "return_terminated cd" by simp
-  with 4 Y have "unflatten_code (?code' @ flatten_code' (length ?code') cd
-    (BPushLam (length lib + length (flatten_code' (length lib) cd' [])) # acc))
+  let ?code' = "lib @ flatten_code' (length lib) cd' r' []"
+  let ?code = "?code' @ flatten_code' ?pc cd r (BPushLam ?pc # acc)"
+  have "length lib + length (flatten_code' (length lib) cd' r' []) = length ?code'" by simp
+  with 5 have "unflatten_return (?code' @ flatten_code' (length ?code') cd r 
+    (BPushLam (length lib + length (flatten_code' (length lib) cd' r' [])) # acc))
+     (length ?code' + code_list_size cd) = r" by blast
+  hence "unflatten_return ?code (length lib + code_list_size cd' + code_list_size cd) = r" by simp
+  hence "unflatten_return ?code (length lib + (code_list_size cd' + code_list_size cd)) = r" 
+    by (metis add.assoc)
+  thus ?case by simp
+qed simp_all
+
+lemma unflatten_flatten [simp]: "unflatten_code (lib @ flatten_code' (length lib) cd r acc) 
+  (length lib + code_list_size cd) = cd"
+proof (induction "length lib" cd r acc arbitrary: lib rule: flatten_code'.induct)
+  case (5 cd' r' cd r acc)
+  let ?pc = "length lib + code_list_size cd'"
+  let ?code' = "lib @ flatten_code' (length lib) cd' r' []"
+  let ?code = "?code' @ flatten_code' ?pc cd r (BPushLam ?pc # acc)"
+  have "length lib + length (flatten_code' (length lib) cd' r' []) = length ?code'" by simp
+  with 5 have "unflatten_code (?code' @ flatten_code' (length ?code') cd r
+    (BPushLam (length lib + length (flatten_code' (length lib) cd' r' [])) # acc))
       (length ?code' + code_list_size cd) = cd" by blast
   hence "unflatten_code ?code (length lib + code_list_size cd' + code_list_size cd) = cd" by simp
   hence X: "unflatten_code ?code (length lib + (code_list_size cd' + code_list_size cd)) = cd" 
     by (metis add.assoc)
-  have "?pc \<le> length ?code'" by simp
-  moreover from 4 have "unflatten_code ?code' (length lib + code_list_size cd') = cd'" by simp
-  ultimately have "unflatten_code (?code' @ flatten_code' ?pc cd (BPushLam ?pc # acc)) ?pc =  cd'" 
-    by (metis unflatten_front)
-  with X show ?case by simp
-next
-  case (6 cd acc)
-  moreover have "(lib @ BReturn # acc) ! length lib = BReturn" by simp
-  ultimately show ?case by simp
-next
-  case (7 cd acc)
-  moreover have "(lib @ BJump # acc) ! length lib = BJump" by simp
-  ultimately show ?case by simp
+  have P: "?pc \<le> length ?code'" by simp
+  moreover from 5 have "unflatten_code ?code' (length lib + code_list_size cd') = cd'" by simp
+  ultimately have Z: "unflatten_code ?code ?pc =  cd'" by (metis unflatten_front)
+  from P have "unflatten_return ?code ?pc = unflatten_return ?code' ?pc" 
+    by (metis unflatten_r_front)
+  with X Z show ?case by simp
 qed simp_all
 
-lemma [simp]: "return_terminated cd \<Longrightarrow> unflatten_code (flatten_code cd) (code_list_size cd) = cd"
-proof (unfold flatten_code_def)
-  assume "return_terminated cd"
-  hence "unflatten_code ([] @ flatten_code' (length []) cd []) (length [] + code_list_size cd) = cd" 
-    by (metis unflatten_flatten list.size(3))
-  thus "unflatten_code (flatten_code' 0 cd []) (code_list_size cd) = cd" by simp
+lemma [simp]: "unflatten_return (flatten_code (cd, r)) (code_list_size cd) = r"
+proof -
+  have "unflatten_return ([] @ flatten_code' (length []) cd r []) (length [] + code_list_size cd) = 
+    r" by (metis unflatten_flatten_r list.size(3))
+  thus ?thesis by simp
 qed
 
-lemma orderly_lam [simp]: "Suc pc \<le> length cd \<Longrightarrow> cd ! pc = BPushLam pc' \<Longrightarrow> orderly cd n \<Longrightarrow> 
+lemma [simp]: "unflatten_code (flatten_code (cd, r)) (code_list_size cd) = cd"
+proof -
+  have "unflatten_code ([] @ flatten_code' (length []) cd r []) 
+    (length [] + code_list_size cd) = cd" by (metis unflatten_flatten list.size(3))
+  thus ?thesis by simp
+qed
+
+lemma orderly_lam [simp]: "pc < length cd \<Longrightarrow> cd ! pc = BPushLam pc' \<Longrightarrow> orderly cd n \<Longrightarrow> 
     pc' \<le> pc + n"
   by (induction cd pc arbitrary: n rule: lookup.induct) fastforce+
 
-lemma [simp]: "Suc pc \<le> length cd \<Longrightarrow> cd ! pc = BPushLam pc' \<Longrightarrow> orderly cd 0 \<Longrightarrow> pc' \<le> pc"
+lemma [simp]: "pc < length cd \<Longrightarrow> cd ! pc = BPushLam pc' \<Longrightarrow> orderly cd 0 \<Longrightarrow> pc' \<le> pc"
   using orderly_lam by fastforce
-
-*)
 
 theorem correctb [simp]: "\<Sigma>\<^sub>b \<leadsto>\<^sub>b \<Sigma>\<^sub>b' \<Longrightarrow> orderly_state \<Sigma>\<^sub>b \<Longrightarrow> 
   iter (\<leadsto>\<^sub>t\<^sub>c\<^sub>o) (unflatten_state \<Sigma>\<^sub>b) (unflatten_state \<Sigma>\<^sub>b')"
-  by simp
-(*
 proof (induction \<Sigma>\<^sub>b \<Sigma>\<^sub>b' rule: evalb.induct)
-  case (evb_lookup cd pc x env v vs envs pcs)
-  hence "TS (ufcs cd vs) (ufcs cd env # map (ufcs cd) envs) 
-    (unflatten_code cd (Suc pc) @ ufcd cd pcs) \<leadsto>\<^sub>t
-      TS (unflatten_closure cd v # ufcs cd vs) (map (ufcs cd) envs) 
-        (unflatten_code cd pc @ ufcd cd pcs)" by simp
+  case (evb_lookup cd pc x env v vs sfs)
+  hence "TCOS (ufcs cd vs) 
+    ((ufcs cd env, unflatten_code cd (Suc pc), unflatten_return cd (Suc pc)) # ufsfs cd sfs) \<leadsto>\<^sub>t\<^sub>c\<^sub>o
+      TCOS (unflatten_closure cd v # ufcs cd vs)
+        ((ufcs cd env, unflatten_code cd pc, unflatten_return cd pc) # ufsfs cd sfs)" by simp
   thus ?case by simp
 next
-  case (evb_pushcon cd pc k vs env envs pcs)
-  hence "TS (ufcs cd vs) (ufcs cd env # map (ufcs cd) envs) 
-    (unflatten_code cd (Suc pc) @ ufcd cd pcs) \<leadsto>\<^sub>t
-      TS (TConst k # ufcs cd vs) (map (ufcs cd) envs) (unflatten_code cd pc @ ufcd cd pcs)" by simp
+  case (evb_pushcon cd pc k vs env sfs)
+  hence "TCOS (ufcs cd vs) 
+    ((ufcs cd env, unflatten_code cd (Suc pc), unflatten_return cd (Suc pc)) # ufsfs cd sfs) \<leadsto>\<^sub>t\<^sub>c\<^sub>o
+      TCOS (TCOConst k # ufcs cd vs) 
+        ((ufcs cd env, unflatten_code cd pc, unflatten_return cd pc) # ufsfs cd sfs)" by simp
   thus ?case by simp
 next
-  case (evb_pushlam cd pc pc' vs env envs pcs)
+  case (evb_pushlam cd pc pc' vs env sfs)
   moreover hence "pc' \<le> pc" by auto
-  moreover have "iter (\<leadsto>\<^sub>t) (TS (ufcs cd vs) (ufcs cd env # map (ufcs cd) envs)
-    (TPushLam (unflatten_code cd pc') # unflatten_code cd pc @ ufcd cd pcs))
-      (TS (TLam (ufcs cd env) (unflatten_code cd pc') # ufcs cd vs) (map (ufcs cd) envs)
-        (unflatten_code cd pc @ ufcd cd pcs))" by (metisx evt_pushlam iter_step iter_refl)
+  moreover have "iter (\<leadsto>\<^sub>t\<^sub>c\<^sub>o) (TCOS (ufcs cd vs) ((ufcs cd env, 
+    TCOPushLam (unflatten_code cd pc') (unflatten_return cd pc') # unflatten_code cd pc, 
+      unflatten_return cd pc) # ufsfs cd sfs))
+        (TCOS (TCOLam (ufcs cd env) (unflatten_code cd pc') (unflatten_return cd pc') # ufcs cd vs) 
+          ((ufcs cd env, unflatten_code cd pc, unflatten_return cd pc) # ufsfs cd sfs))" 
+    by (metis evtco_pushlam iter_one)
   ultimately show ?case by simp
 next
-  case (evb_enter cd pc vs env envs pcs)
-  hence "TS (ufcs cd vs) (ufcs cd env # map (ufcs cd) envs) 
-    (unflatten_code cd (Suc pc) @ ufcd cd pcs) \<leadsto>\<^sub>t
-      TS (ufcs cd vs) (ufcs cd env # ufcs cd env # map (ufcs cd) envs) 
-        (unflatten_code cd pc @ ufcd cd pcs)" by simp
+  case (evb_apply cd pc v env' pc' vs env sfs)
+  hence "TCOS (unflatten_closure cd v # TCOLam (ufcs cd env') (unflatten_code cd pc') 
+    (unflatten_return cd pc') # ufcs cd vs) 
+      ((ufcs cd env, unflatten_code cd (Suc pc), unflatten_return cd (Suc pc)) # ufsfs cd sfs) \<leadsto>\<^sub>t\<^sub>c\<^sub>o
+        TCOS (ufcs cd vs) ((unflatten_closure cd v # ufcs cd env', unflatten_code cd pc', 
+          unflatten_return cd pc') # (ufcs cd env, unflatten_code cd pc, unflatten_return cd pc) # 
+            ufsfs cd sfs)" by simp
   thus ?case by simp
 next
-  case (evb_apply cd pc v env pc' vs envs pcs)
-  hence "TS (unflatten_closure cd v # TLam (ufcs cd env) (unflatten_code cd pc') # ufcs cd vs) 
-    (map (ufcs cd) envs) (unflatten_code cd (Suc pc) @ ufcd cd pcs) \<leadsto>\<^sub>t
-      TS (ufcs cd vs) ((unflatten_closure cd v # ufcs cd env) # map (ufcs cd) envs)
-        (unflatten_code cd pc' @ unflatten_code cd pc @ ufcd cd pcs)" by simp
+  case (evb_return cd pc vs env sfs)
+  hence "TCOS (ufcs cd vs) 
+    ((ufcs cd env, unflatten_code cd (Suc pc), unflatten_return cd (Suc pc)) # ufsfs cd sfs) \<leadsto>\<^sub>t\<^sub>c\<^sub>o
+      TCOS (ufcs cd vs) (ufsfs cd sfs)" by simp
   thus ?case by simp
 next
-  case (evb_returnb cd pc vs env envs pcs)
-  hence "TS (ufcs cd vs) (ufcs cd env # map (ufcs cd) envs) 
-    (unflatten_code cd (Suc pc) @ ufcd cd pcs) \<leadsto>\<^sub>t 
-      TS (ufcs cd vs) (map (ufcs cd) envs) (ufcd cd pcs)" by simp
-  thus ?case by simp
-next
-  case (evb_jump cd pc v env' pc' vs env envs pcs)
-  hence "TS (unflatten_closure cd v # TLam (ufcs cd env') (unflatten_code cd pc') # ufcs cd vs)
-    (ufcs cd env # map (ufcs cd) envs) (unflatten_code cd (Suc pc) @ ufcd cd pcs) \<leadsto>\<^sub>t
-      TS (ufcs cd vs) ((unflatten_closure cd v # ufcs cd env') # map (ufcs cd) envs)
-        (unflatten_code cd pc' @ ufcd cd pcs)" by simp
-  hence "iter (\<leadsto>\<^sub>t) (TS (unflatten_closure cd v # TLam (ufcs cd env') (unflatten_code cd pc') # 
-    ufcs cd vs) (ufcs cd env # map (ufcs cd) envs) (unflatten_code cd (Suc pc) @ ufcd cd pcs))
-      (TS (ufcs cd vs) ((unflatten_closure cd v # ufcs cd env') # map (ufcs cd) envs)
-        (unflatten_code cd pc' @ ufcd cd pcs))" using iter_step iter_refl by fast
-  thus ?case by simp
-qed simp_all
-
-lemma [simp]: "TLam envt cdt = unflatten_closure cdb vb \<Longrightarrow> 
-    \<exists>envb pc. vb = BLam envb pc \<and> envt = ufcs cdb envb \<and> cdt = unflatten_code cdb pc"
-  by (induction vb) simp_all
-
-lemma unfl_state [simp]: "TS vs envs cd = unflatten_state \<Sigma>\<^sub>b \<Longrightarrow> \<exists>vsb envsb pcs cdb. 
-    \<Sigma>\<^sub>b = BS vsb envsb pcs cdb \<and> vs = ufcs cdb vsb \<and> envs = map (ufcs cdb) envsb \<and> cd = ufcd cdb pcs"
-  by (induction \<Sigma>\<^sub>b) simp_all
-
-lemma unfl_tlu [simp]: "TLookup x # cdt = unflatten_code cdb (Suc pc) @ cdt' \<Longrightarrow> orderly cdb 0 \<Longrightarrow> 
-  Suc pc \<le> length cdb \<Longrightarrow> (cdb ! pc = BLookup x \<and> cdt = unflatten_code cdb pc @ cdt')
-    \<or> (cdb ! pc = BReturn_Old \<and> cdt' = TLookup x # cdt)"
-  by (cases "cdb ! pc") simp_all
-
-lemma unfl_tpc [simp]: "TPushCon k # cdt = unflatten_code cdb (Suc pc) @ cdt' \<Longrightarrow> orderly cdb 0 \<Longrightarrow> 
-  Suc pc \<le> length cdb \<Longrightarrow> (cdb ! pc = BPushCon k \<and> cdt = unflatten_code cdb pc @ cdt')
-    \<or> (cdb ! pc = BReturn_Old \<and> cdt' = TPushCon k # cdt)"
-  by (cases "cdb ! pc") simp_all
-
-lemma unfl_tpl [simp]: "TPushLam cdt'' # cdt = unflatten_code cdb (Suc pc) @ cdt' \<Longrightarrow> 
-  orderly cdb 0 \<Longrightarrow> Suc pc \<le> length cdb \<Longrightarrow> 
-    (\<exists>pc'. cdb ! pc = BPushLam pc' \<and> cdt = unflatten_code cdb pc @ cdt' \<and> 
-      cdt'' = unflatten_code cdb pc') \<or> (cdb ! pc = BReturn_Old \<and> cdt' = TPushLam cdt'' # cdt)"
-  by (cases "cdb ! pc") simp_all
-
-lemma unfl_te [simp]: "TEnter # cdt = unflatten_code cdb (Suc pc) @ cdt' \<Longrightarrow> orderly cdb 0 \<Longrightarrow> 
-  Suc pc \<le> length cdb \<Longrightarrow> (cdb ! pc = BEnter \<and> cdt = unflatten_code cdb pc @ cdt')
-    \<or> (cdb ! pc = BReturn_Old \<and> cdt' = TEnter # cdt)"
-  by (cases "cdb ! pc") simp_all
-
-lemma unfl_ta [simp]: "TApply # cdt = unflatten_code cdb (Suc pc) @ cdt' \<Longrightarrow> orderly cdb 0 \<Longrightarrow> 
-  Suc pc \<le> length cdb \<Longrightarrow> (cdb ! pc = BApply \<and> cdt = unflatten_code cdb pc @ cdt')
-    \<or> (cdb ! pc = BReturn_Old \<and> cdt' = TApply # cdt)"
-  by (cases "cdb ! pc") simp_all
-
-abbreviation poppable :: "byte_code list \<Rightarrow> nat list \<Rightarrow> bool" where
-  "poppable cd rs \<equiv> (\<forall>r \<in> set rs. \<exists>r'. r = Suc r' \<and> cd ! r' = BReturn_Old)"
-
-lemma [simp]: "TLookup x # cdt = ufcd cdb pcs \<Longrightarrow> orderly cdb 0 \<Longrightarrow> 
-  \<forall>pc \<in> set pcs. pc \<le> length cdb \<and> pc \<noteq> 0 \<Longrightarrow> \<exists>rs pc pcs'. pcs = rs @ Suc pc # pcs' \<and> 
-    poppable cdb rs \<and> cdb ! pc = BLookup x \<and> cdt = unflatten_code cdb pc @ ufcd cdb pcs'"
-proof (induction pcs)
-  case (Cons pc pcs)
-  thus ?case
-  proof (induction pc)
-    case (Suc pc)
-    show ?case
-    proof (cases "cdb ! pc = BLookup x \<and> cdt = unflatten_code cdb pc @ ufcd cdb pcs")
-      case False
-      moreover from Suc have "TLookup x # cdt = unflatten_code cdb (Suc pc) @ ufcd cdb pcs" by simp
-      moreover from Suc have "orderly cdb 0" by simp
-      moreover from Suc have "Suc pc \<le> length cdb" by simp
-      ultimately have X: "cdb ! pc = BReturn_Old \<and> ufcd cdb pcs = TLookup x # cdt" by (metis unfl_tlu)
-      from Suc have "\<forall>pc\<in>set pcs. pc \<le> length cdb \<and> pc \<noteq> 0" by simp
-      with Suc X obtain rs pc' pcs' where "pcs = rs @ Suc pc' # pcs' \<and> poppable cdb rs \<and> 
-        cdb ! pc' = BLookup x \<and> cdt = unflatten_code cdb pc' @ ufcd cdb pcs'" by metis
-      with X have "Suc pc # pcs = (Suc pc # rs) @ Suc pc' # pcs' \<and> poppable cdb (Suc pc # rs) \<and> 
-        cdb ! pc' = BLookup x \<and> cdt = unflatten_code cdb pc' @ ufcd cdb pcs'" by simp
-      thus ?thesis by blast
-    qed fastforcex+
-  qed simp_all
-qed simp_all
-
-lemma [simp]: "TPushCon k # cdt = ufcd cdb pcs \<Longrightarrow> orderly cdb 0 \<Longrightarrow> 
-  \<forall>pc \<in> set pcs. pc \<le> length cdb \<and> pc \<noteq> 0 \<Longrightarrow> \<exists>rs pc pcs'. pcs = rs @ Suc pc # pcs' \<and> 
-    poppable cdb rs \<and> cdb ! pc = BPushCon k \<and> cdt = unflatten_code cdb pc @ ufcd cdb pcs'"
-proof (induction pcs)
-  case (Cons pc pcs)
-  thus ?case
-  proof (induction pc)
-    case (Suc pc)
-    show ?case
-    proof (cases "cdb ! pc = BPushCon k \<and> cdt = unflatten_code cdb pc @ ufcd cdb pcs")
-      case False
-      moreover from Suc have "TPushCon k # cdt = unflatten_code cdb (Suc pc) @ ufcd cdb pcs" by simp
-      moreover from Suc have "orderly cdb 0" by simp
-      moreover from Suc have "Suc pc \<le> length cdb" by simp
-      ultimately have X: "cdb ! pc = BReturn_Old \<and> ufcd cdb pcs = TPushCon k # cdt" by (metis unfl_tpc)
-      from Suc have "\<forall>pc\<in>set pcs. pc \<le> length cdb \<and> pc \<noteq> 0" by simp
-      with Suc X obtain rs pc' pcs' where "pcs = rs @ Suc pc' # pcs' \<and> poppable cdb rs \<and> 
-        cdb ! pc' = BPushCon k \<and> cdt = unflatten_code cdb pc' @ ufcd cdb pcs'" by metis
-      with X have "Suc pc # pcs = (Suc pc # rs) @ Suc pc' # pcs' \<and> poppable cdb (Suc pc # rs) \<and> 
-        cdb ! pc' = BPushCon k \<and> cdt = unflatten_code cdb pc' @ ufcd cdb pcs'" by simp
-      thus ?thesis by blast
-    qed fastforcex+
-  qed simp_all
-qed simp_all
-
-lemma ufcd_pl [simp]: "TPushLam cdt' # cdt = ufcd cdb pcs \<Longrightarrow> orderly cdb 0 \<Longrightarrow> 
-  \<forall>pc \<in> set pcs. pc \<le> length cdb \<and> pc \<noteq> 0 \<Longrightarrow> \<exists>rs pc pcs' pc'. pcs = rs @ Suc pc # pcs' \<and> 
-    poppable cdb rs \<and> cdb ! pc = BPushLam pc' \<and> cdt' = unflatten_code cdb pc' \<and> 
-      cdt = unflatten_code cdb pc @ ufcd cdb pcs'"
-proof (induction pcs)
-  case (Cons pc pcs)
-  thus ?case
-  proof (induction pc)
-    case (Suc pc)
-    show ?case
-    proof (cases "\<exists>pc'. cdb ! pc = BPushLam pc' \<and> cdt = unflatten_code cdb pc @ ufcd cdb pcs \<and> 
-                  cdt' = unflatten_code cdb pc'")
-      case False
-      moreover from Suc have "TPushLam cdt' # cdt = unflatten_code cdb (Suc pc) @ ufcd cdb pcs" 
-        by simp
-      moreover from Suc have "orderly cdb 0" by simp
-      moreover from Suc have "Suc pc \<le> length cdb" by simp
-      ultimately have X: "cdb ! pc = BReturn_Old \<and> ufcd cdb pcs = TPushLam cdt' # cdt" 
-        by (metisx unfl_tpl)
-      from Suc have "\<forall>pc\<in>set pcs. pc \<le> length cdb \<and> pc \<noteq> 0" by simp
-      with Suc X obtain rs pca pcs' pc' where "pcs = rs @ Suc pca # pcs' \<and> poppable cdb rs \<and>
-       cdb ! pca = BPushLam pc' \<and> cdt' = unflatten_code cdb pc' \<and> 
-        cdt = unflatten_code cdb pca @ ufcd cdb pcs'" by metis
-      with X have "Suc pc # pcs = (Suc pc # rs) @ Suc pca # pcs' \<and> poppable cdb (Suc pc # rs) \<and> 
-        cdb ! pca = BPushLam pc' \<and> cdt' = unflatten_code cdb pc' \<and> 
-          cdt = unflatten_code cdb pca @ ufcd cdb pcs'" by simp
-      thus ?thesis by blast
-    qed fastforcex+
-  qed simp_all
-qed simp_all
-
-lemma [simp]: "TEnter # cdt = ufcd cdb pcs \<Longrightarrow> orderly cdb 0 \<Longrightarrow> 
-  \<forall>pc \<in> set pcs. pc \<le> length cdb \<and> pc \<noteq> 0 \<Longrightarrow> \<exists>rs pc pcs'. pcs = rs @ Suc pc # pcs' \<and> 
-    poppable cdb rs \<and> cdb ! pc = BEnter \<and> cdt = unflatten_code cdb pc @ ufcd cdb pcs'"
-proof (induction pcs)
-  case (Cons pc pcs)
-  thus ?case
-  proof (induction pc)
-    case (Suc pc)
-    show ?case
-    proof (cases "cdb ! pc = BEnter \<and> cdt = unflatten_code cdb pc @ ufcd cdb pcs")
-      case False
-      moreover from Suc have "TEnter # cdt = unflatten_code cdb (Suc pc) @ ufcd cdb pcs" by simp
-      moreover from Suc have "orderly cdb 0" by simp
-      moreover from Suc have "Suc pc \<le> length cdb" by simp
-      ultimately have X: "cdb ! pc = BReturn_Old \<and> ufcd cdb pcs = TEnter # cdt" by (metis unfl_te)
-      from Suc have "\<forall>pc\<in>set pcs. pc \<le> length cdb \<and> pc \<noteq> 0" by simp
-      with Suc X obtain rs pc' pcs' where "pcs = rs @ Suc pc' # pcs' \<and> poppable cdb rs \<and> 
-        cdb ! pc' = BEnter \<and> cdt = unflatten_code cdb pc' @ ufcd cdb pcs'" by metis
-      with X have "Suc pc # pcs = (Suc pc # rs) @ Suc pc' # pcs' \<and> poppable cdb (Suc pc # rs) \<and> 
-        cdb ! pc' = BEnter \<and> cdt = unflatten_code cdb pc' @ ufcd cdb pcs'" by simp
-      thus ?thesis by blast
-    qed fastforcex+
-  qed simp_all
-qed simp_all
-
-lemma [simp]: "TApply # cdt = ufcd cdb pcs \<Longrightarrow> orderly cdb 0 \<Longrightarrow> 
-  \<forall>pc \<in> set pcs. pc \<le> length cdb \<and> pc \<noteq> 0 \<Longrightarrow> \<exists>rs pc pcs'. pcs = rs @ Suc pc # pcs' \<and> 
-    poppable cdb rs \<and> cdb ! pc = BApply \<and> cdt = unflatten_code cdb pc @ ufcd cdb pcs'"
-proof (induction pcs)
-  case (Cons pc pcs)
-  thus ?case
-  proof (induction pc)
-    case (Suc pc)
-    show ?case
-    proof (cases "cdb ! pc = BApply \<and> cdt = unflatten_code cdb pc @ ufcd cdb pcs")
-      case False
-      moreover from Suc have "TApply # cdt = unflatten_code cdb (Suc pc) @ ufcd cdb pcs" by simp
-      moreover from Suc have "orderly cdb 0" by simp
-      moreover from Suc have "Suc pc \<le> length cdb" by simp
-      ultimately have X: "cdb ! pc = BReturn_Old \<and> ufcd cdb pcs = TApply # cdt" by (metis unfl_ta)
-      from Suc have "\<forall>pc\<in>set pcs. pc \<le> length cdb \<and> pc \<noteq> 0" by simp
-      with Suc X obtain rs pc' pcs' where "pcs = rs @ Suc pc' # pcs' \<and> poppable cdb rs \<and> 
-        cdb ! pc' = BApply \<and> cdt = unflatten_code cdb pc' @ ufcd cdb pcs'" by metis
-      with X have "Suc pc # pcs = (Suc pc # rs) @ Suc pc' # pcs' \<and> poppable cdb (Suc pc # rs) \<and> 
-        cdb ! pc' = BApply \<and> cdt = unflatten_code cdb pc' @ ufcd cdb pcs'" by simp
-      thus ?thesis by blast
-    qed fastforcex+
-  qed simp_all
-qed simp_all
-
-lemma ev_poppable [simp]: "poppable cdb rs \<Longrightarrow> 
-  iter (\<leadsto>\<^sub>b) (BS vs envs (rs @ pcs) cdb) (BS vs envs pcs cdb)"
-proof (induction rs)
-  case (Cons r rs)
-  then obtain r' where "r = Suc r' \<and> cdb ! r' = BReturn_Old" by fastforce
-  hence "BS vs envs (r # rs @ pcs) cdb \<leadsto>\<^sub>b BS vs envs (rs @ pcs) cdb" by simp
-  moreover from Cons have "iter (\<leadsto>\<^sub>b) (BS vs envs (rs @ pcs) cdb) (BS vs envs pcs cdb)" by simp
-  ultimately show ?case by simp
-qed simp_all
-
-*)
-
-theorem completeb [simp]: "unflatten_state \<Sigma>\<^sub>b \<leadsto>\<^sub>t\<^sub>c\<^sub>o \<Sigma>\<^sub>t' \<Longrightarrow> orderly_state \<Sigma>\<^sub>b \<Longrightarrow>
-  \<exists>\<Sigma>\<^sub>b'. iter (\<leadsto>\<^sub>b) \<Sigma>\<^sub>b \<Sigma>\<^sub>b' \<and> unflatten_state \<Sigma>\<^sub>b' = \<Sigma>\<^sub>t'"
-  by simp
-(*
-proof (induction "unflatten_state \<Sigma>\<^sub>b" \<Sigma>\<^sub>t' rule: evalt.induct)
-  case (evt_lookup env x v vs envs cd)
-  then obtain vsb envsb pcs cdb where S: "\<Sigma>\<^sub>b = BS vsb envsb pcs cdb \<and> vs = ufcs cdb vsb \<and> 
-    env # envs = map (ufcs cdb) envsb \<and> TLookup x # cd = ufcd cdb pcs" by fastforce
-  then obtain envb envsb' where E: "envsb = envb # envsb' \<and> env = ufcs cdb envb \<and> 
-    envs = map (ufcs cdb) envsb'" by fastforce
-  from S evt_lookup obtain rs pc pcs' where R: "pcs = rs @ Suc pc # pcs' \<and> poppable cdb rs \<and> 
-    cdb ! pc = BLookup x \<and> cd = unflatten_code cdb pc @ ufcd cdb pcs'" by fastforce
-  hence X: "iter (\<leadsto>\<^sub>b) (BS vsb (envb # envsb') (rs @ Suc pc # pcs') cdb) 
-    (BS vsb (envb # envsb') (Suc pc # pcs') cdb)" by simp
-  from evt_lookup E obtain vb where V: "lookup envb x = Some vb \<and> unflatten_closure cdb vb = v" 
-    by fastforce
-  with R have "BS vsb (envb # envsb') (Suc pc # pcs') cdb \<leadsto>\<^sub>b 
-    BS (vb # vsb) envsb' (pc # pcs') cdb" by simp
-  with X have "iter (\<leadsto>\<^sub>b) (BS vsb (envb # envsb') (rs @ Suc pc # pcs') cdb) 
-    (BS (vb # vsb) envsb' (pc # pcs') cdb)" by simp
-  with S E R V show ?case by fastforcex
-next
-  case (evt_pushcon vs env envs k cd)
-  then obtain vsb envsb pcs cdb where S: "\<Sigma>\<^sub>b = BS vsb envsb pcs cdb \<and> vs = ufcs cdb vsb \<and> 
-    env # envs = map (ufcs cdb) envsb \<and> TPushCon k # cd = ufcd cdb pcs" by fastforce
-  then obtain envb envsb' where E: "envsb = envb # envsb' \<and> env = ufcs cdb envb \<and> 
-    envs = map (ufcs cdb) envsb'" by fastforce
-  from S evt_pushcon obtain rs pc pcs' where R: "pcs = rs @ Suc pc # pcs' \<and> poppable cdb rs \<and> 
-    cdb ! pc = BPushCon k \<and> cd = unflatten_code cdb pc @ ufcd cdb pcs'" by fastforcex
-  hence "iter (\<leadsto>\<^sub>b) (BS vsb (envb # envsb') (rs @ Suc pc # pcs') cdb) 
-    (BS vsb (envb # envsb') (Suc pc # pcs') cdb)" by simp
-  moreover from R have "BS vsb (envb # envsb') (Suc pc # pcs') cdb \<leadsto>\<^sub>b 
-    BS (BConst k # vsb) envsb' (pc # pcs') cdb" by simp
-  ultimately have "iter (\<leadsto>\<^sub>b) (BS vsb (envb # envsb') (rs @ Suc pc # pcs') cdb) 
-    (BS (BConst k # vsb) envsb' (pc # pcs') cdb)" by simp
-  with S E R show ?case by fastforce
-next
-  case (evt_pushlam vs env envs cd' cd)
-  then obtain vsb envsb pcs cdb where S: "\<Sigma>\<^sub>b = BS vsb envsb pcs cdb \<and> vs = ufcs cdb vsb \<and> 
-    env # envs = map (ufcs cdb) envsb \<and> TPushLam cd' # cd = ufcd cdb pcs" by fastforcex
-  then obtain envb envsb' where E: "envsb = envb # envsb' \<and> env = ufcs cdb envb \<and> 
-    envs = map (ufcs cdb) envsb'" by fastforce
-  from S evt_pushlam obtain rs pc pcs' pc' where R: "pcs = rs @ Suc pc # pcs' \<and> poppable cdb rs \<and> 
-    cdb ! pc = BPushLam pc' \<and> cd' = unflatten_code cdb pc' \<and> 
-      cd = unflatten_code cdb pc @ ufcd cdb pcs'" using ufcd_pl by fastforcex
-  hence "iter (\<leadsto>\<^sub>b) (BS vsb (envb # envsb') (rs @ Suc pc # pcs') cdb) 
-    (BS vsb (envb # envsb') (Suc pc # pcs') cdb)" by simp
-  moreover from R have "BS vsb (envb # envsb') (Suc pc # pcs') cdb \<leadsto>\<^sub>b 
-    BS (BLam envb pc' # vsb) envsb' (pc # pcs') cdb" by simp
-  ultimately have "iter (\<leadsto>\<^sub>b) (BS vsb (envb # envsb') (rs @ Suc pc # pcs') cdb) 
-    (BS (BLam envb pc' # vsb) envsb' (pc # pcs') cdb)" by simp
-  with S E R show ?case by fastforce
-next
-  case (evt_enter vs env envs cd)
-  then obtain vsb envsb pcs cdb where S: "\<Sigma>\<^sub>b = BS vsb envsb pcs cdb \<and> vs = ufcs cdb vsb \<and> 
-    env # envs = map (ufcs cdb) envsb \<and> TEnter # cd = ufcd cdb pcs" by fastforcex
-  then obtain envb envsb' where E: "envsb = envb # envsb' \<and> env = ufcs cdb envb \<and> 
-    envs = map (ufcs cdb) envsb'" by fastforce
-  from S evt_enter obtain rs pc pcs' where R: "pcs = rs @ Suc pc # pcs' \<and> poppable cdb rs \<and> 
-    cdb ! pc = BEnter \<and> cd = unflatten_code cdb pc @ ufcd cdb pcs'" by fastforce
-  hence "iter (\<leadsto>\<^sub>b) (BS vsb (envb # envsb') (rs @ Suc pc # pcs') cdb) 
-    (BS vsb (envb # envsb') (Suc pc # pcs') cdb)" by simp
-  moreover from R have "BS vsb (envb # envsb') (Suc pc # pcs') cdb \<leadsto>\<^sub>b 
-    BS vsb (envb # envb # envsb') (pc # pcs') cdb" by simp
-  ultimately have "iter (\<leadsto>\<^sub>b) (BS vsb (envb # envsb') (rs @ Suc pc # pcs') cdb) 
-    (BS vsb (envb # envb # envsb') (pc # pcs') cdb)" by simp
-  with S E R show ?case by fastforce
-next
-  case (evt_apply v env cd' vs envs cd)
-  then obtain vsb envsb pcs cdb where S: "\<Sigma>\<^sub>b = BS vsb envsb pcs cdb \<and> 
-    v # TLam env cd' # vs = ufcs cdb vsb \<and> envs = map (ufcs cdb) envsb \<and> 
-      TApply # cd = ufcd cdb pcs" by fastforcex
-  then obtain vb vvb vsb' where V: "vsb = vb # vvb # vsb' \<and> v = unflatten_closure cdb vb \<and> 
-    TLam env cd' = unflatten_closure cdb vvb \<and> vs = ufcs cdb vsb'" by fastforce
-  then obtain envb pc' where L: "vvb = BLam envb pc' \<and> env = ufcs cdb envb \<and> 
-    cd' = unflatten_code cdb pc'" by fastforce
-  from S evt_apply obtain rs pc pcs' where R: "pcs = rs @ Suc pc # pcs' \<and> poppable cdb rs \<and> 
-    cdb ! pc = BApply \<and> cd = unflatten_code cdb pc @ ufcd cdb pcs'" by fastforcex
-  hence "iter (\<leadsto>\<^sub>b) (BS (vb # BLam envb pc' # vsb') envsb (rs @ Suc pc # pcs') cdb) 
-    (BS (vb # BLam envb pc' # vsb') envsb (Suc pc # pcs') cdb)" by simp
-  moreover from R have "BS (vb # BLam envb pc' # vsb') envsb (Suc pc # pcs') cdb \<leadsto>\<^sub>b 
-    BS vsb' ((vb # envb) # envsb) (pc' # pc # pcs') cdb" by simp
-  ultimately have X: "iter (\<leadsto>\<^sub>b) (BS (vb # BLam envb pc' # vsb') envsb (rs @ Suc pc # pcs') cdb) 
-    (BS vsb' ((vb # envb) # envsb) (pc' # pc # pcs') cdb)" by simp
-  from S V L R have "unflatten_state (BS vsb' ((vb # envb) # envsb) (pc' # pc # pcs') cdb) = 
-    TS vs ((v # env) # envs) (cd' @ cd)" by simp
-  with S V L R X show ?case by blast
-next
-  case evt_return
-  thus ?case by simp
-next
-  case evt_jump
+  case (evb_jump cd pc v env' pc' vs env sfs)
+  hence "TCOS (unflatten_closure cd v # 
+    TCOLam (ufcs cd env') (unflatten_code cd pc') (unflatten_return cd pc') # ufcs cd vs)
+      ((ufcs cd env, unflatten_code cd (Suc pc), unflatten_return cd (Suc pc)) # ufsfs cd sfs) \<leadsto>\<^sub>t\<^sub>c\<^sub>o
+        TCOS (ufcs cd vs) ((unflatten_closure cd v # ufcs cd env', unflatten_code cd pc', 
+          unflatten_return cd pc') # ufsfs cd sfs)" by simp
+  hence "iter (\<leadsto>\<^sub>t\<^sub>c\<^sub>o) (TCOS (unflatten_closure cd v # 
+    TCOLam (ufcs cd env') (unflatten_code cd pc') (unflatten_return cd pc') # ufcs cd vs)
+      ((ufcs cd env, unflatten_code cd (Suc pc), unflatten_return cd (Suc pc)) # ufsfs cd sfs))
+        (TCOS (ufcs cd vs) ((unflatten_closure cd v # ufcs cd env', unflatten_code cd pc', 
+          unflatten_return cd pc') # ufsfs cd sfs))" by (metis iter_one)
   thus ?case by simp
 qed
 
-*)
+lemma [simp]: "TCOLam envt cdt rt = unflatten_closure cdb vb \<Longrightarrow> 
+  \<exists>envb pc. vb = BLam envb pc \<and> envt = ufcs cdb envb \<and> cdt = unflatten_code cdb pc \<and>
+    rt = unflatten_return cdb pc"
+  by (induction vb) simp_all
+
+lemma unfl_state [dest]: "TCOS vs sfs = unflatten_state \<Sigma>\<^sub>b \<Longrightarrow> \<exists>vsb sfsb cdb. 
+    \<Sigma>\<^sub>b = BS vsb sfsb cdb \<and> vs = ufcs cdb vsb \<and> sfs = ufsfs cdb sfsb"
+  by (induction \<Sigma>\<^sub>b) simp_all
+
+lemma [dest]: "TCOLookup x # cdt = unflatten_code cdb (Suc pc) \<Longrightarrow> orderly cdb 0 \<Longrightarrow> 
+    pc < length cdb \<Longrightarrow> cdb ! pc = BLookup x \<and> cdt = unflatten_code cdb pc"
+  by (cases "cdb ! pc") simp_all
+
+lemma [dest]: "TCOPushCon k # cdt = unflatten_code cdb (Suc pc) \<Longrightarrow> orderly cdb 0 \<Longrightarrow> 
+    pc < length cdb \<Longrightarrow> cdb ! pc = BPushCon k \<and> cdt = unflatten_code cdb pc"
+  by (cases "cdb ! pc") simp_all
+
+lemma [dest]: "TCOPushLam cdt'' r # cdt = unflatten_code cdb (Suc pc) \<Longrightarrow> 
+  orderly cdb 0 \<Longrightarrow> pc < length cdb \<Longrightarrow> 
+    \<exists>pc'. cdb ! pc = BPushLam pc' \<and> cdt = unflatten_code cdb pc \<and> 
+      cdt'' = unflatten_code cdb pc' \<and> r = unflatten_return cdb pc'"
+  by (cases "cdb ! pc") simp_all
+
+lemma [dest]: "TCOApply # cdt = unflatten_code cdb (Suc pc) \<Longrightarrow> orderly cdb 0 \<Longrightarrow> 
+    pc < length cdb \<Longrightarrow> cdb ! pc = BApply \<and> cdt = unflatten_code cdb pc"
+  by (cases "cdb ! pc") simp_all
+
+lemma uf_to_lookup [dest]: "(envt, TCOLookup x # cdt, r) # sfst = ufsfs cdb sfsb \<Longrightarrow> 
+  orderly cdb 0 \<Longrightarrow> orderly_stack sfsb (length cdb) \<Longrightarrow> \<exists>envb pc sfsb'. 
+    sfsb = (envb, Suc pc) # sfsb' \<and> envt = ufcs cdb envb \<and> cdb ! pc = BLookup x \<and> 
+      cdt = unflatten_code cdb pc \<and> r = unflatten_return cdb pc \<and> sfst = ufsfs cdb sfsb'"
+proof (induction sfsb "length cdb" rule: orderly_stack.induct)
+  case (3 envb pc sfsb')
+  hence "TCOLookup x # cdt = unflatten_code cdb (Suc pc) \<and> orderly cdb 0 \<and> pc < length cdb" by simp
+  hence "cdb ! pc = BLookup x \<and> cdt = unflatten_code cdb pc" by blast
+  with 3 show ?case by simp
+qed simp_all
+
+lemma [dest]: "(envt, TCOPushCon k # cdt, r) # sfst = ufsfs cdb sfsb \<Longrightarrow> orderly cdb 0 \<Longrightarrow> 
+  orderly_stack sfsb (length cdb) \<Longrightarrow> \<exists>envb pc sfsb'. sfsb = (envb, Suc pc) # sfsb' \<and> 
+    envt = ufcs cdb envb \<and> cdb ! pc = BPushCon k \<and> cdt = unflatten_code cdb pc \<and> 
+      r = unflatten_return cdb pc \<and> sfst = ufsfs cdb sfsb'"
+proof (induction sfsb "length cdb" rule: orderly_stack.induct)
+  case (3 envb pc sfsb')
+  hence "TCOPushCon k # cdt = unflatten_code cdb (Suc pc) \<and> orderly cdb 0 \<and> pc < length cdb" by simp
+  hence "cdb ! pc = BPushCon k \<and> cdt = unflatten_code cdb pc" by blast
+  with 3 show ?case by simp
+qed simp_all
+
+lemma [dest]: "(envt, TCOPushLam cdt' r' # cdt, r) # sfst = ufsfs cdb sfsb \<Longrightarrow> 
+  orderly cdb 0 \<Longrightarrow> orderly_stack sfsb (length cdb) \<Longrightarrow> \<exists>envb pc sfsb' pc'. 
+    sfsb = (envb, Suc pc) # sfsb' \<and> envt = ufcs cdb envb \<and> cdb ! pc = BPushLam pc' \<and> 
+      cdt = unflatten_code cdb pc \<and> r = unflatten_return cdb pc \<and> cdt' = unflatten_code cdb pc' \<and> 
+        r' = unflatten_return cdb pc' \<and> sfst = ufsfs cdb sfsb'"
+proof (induction sfsb "length cdb" rule: orderly_stack.induct)
+  case (3 envb pc sfsb')
+  hence "TCOPushLam cdt' r' # cdt = unflatten_code cdb (Suc pc) \<and> orderly cdb 0 \<and> pc < length cdb" 
+    by simp
+  then obtain pc' where "cdb ! pc = BPushLam pc' \<and> cdt = unflatten_code cdb pc \<and> 
+    cdt' = unflatten_code cdb pc' \<and> r' = unflatten_return cdb pc'" by blast
+  with 3 show ?case by simp
+qed simp_all
+
+lemma [dest]: "(envt, TCOApply # cdt, r) # sfst = ufsfs cdb sfsb \<Longrightarrow> orderly cdb 0 \<Longrightarrow> 
+  orderly_stack sfsb (length cdb) \<Longrightarrow> \<exists>envb pc sfsb'. sfsb = (envb, Suc pc) # sfsb' \<and> 
+    envt = ufcs cdb envb \<and> cdb ! pc = BApply \<and> cdt = unflatten_code cdb pc \<and> 
+      r = unflatten_return cdb pc \<and> sfst = ufsfs cdb sfsb'"
+proof (induction sfsb "length cdb" rule: orderly_stack.induct)
+  case (3 envb pc sfsb')
+  hence "TCOApply # cdt = unflatten_code cdb (Suc pc) \<and> orderly cdb 0 \<and> pc < length cdb" by simp
+  hence "cdb ! pc = BApply \<and> cdt = unflatten_code cdb pc" by blast
+  with 3 show ?case by simp
+qed simp_all
+
+theorem completeb [simp]: "unflatten_state \<Sigma>\<^sub>b \<leadsto>\<^sub>t\<^sub>c\<^sub>o \<Sigma>\<^sub>t' \<Longrightarrow> orderly_state \<Sigma>\<^sub>b \<Longrightarrow>
+  \<exists>\<Sigma>\<^sub>b'. iter (\<leadsto>\<^sub>b) \<Sigma>\<^sub>b \<Sigma>\<^sub>b' \<and> unflatten_state \<Sigma>\<^sub>b' = \<Sigma>\<^sub>t'"
+proof (induction "unflatten_state \<Sigma>\<^sub>b" \<Sigma>\<^sub>t' rule: evaltco.induct)
+  case (evtco_lookup env x v vs cd r sfs)
+  then obtain vsb sfsb cdb where B: "\<Sigma>\<^sub>b = BS vsb sfsb cdb \<and> vs = ufcs cdb vsb \<and> 
+    (env, TCOLookup x # cd, r) # sfs = ufsfs cdb sfsb" by fastforce
+  with evtco_lookup have "orderly cdb 0 \<and> orderly_stack sfsb (length cdb)" by simp
+  with B obtain envb pc sfsb' where S: "sfsb = (envb, Suc pc) # sfsb' \<and> 
+    env = ufcs cdb envb \<and> cdb ! pc = BLookup x \<and> cd = unflatten_code cdb pc \<and> 
+      r = unflatten_return cdb pc \<and> sfs = ufsfs cdb sfsb'" by (metis uf_to_lookup)
+  with evtco_lookup obtain v' where V: "lookup envb x = Some v' \<and> unflatten_closure cdb v' = v"
+    by fastforce
+  with S have "BS vsb ((envb, Suc pc) # sfsb') cdb \<leadsto>\<^sub>b BS (v' # vsb) ((envb, pc) # sfsb') cdb"
+    by simp
+  hence "iter (\<leadsto>\<^sub>b) (BS vsb ((envb, Suc pc) # sfsb') cdb) (BS (v' # vsb) ((envb, pc) # sfsb') cdb)" 
+    by simp
+  with B S V show ?case by fastforce
+next
+  case (evtco_pushcon vs env k cd r sfs)
+  then show ?case by simp
+next
+  case (evtco_pushlam vs env cd' r' cd r sfs)
+  then show ?case by simp
+next
+  case (evtco_apply v env' cd' r' vs env cd r sfs)
+  then show ?case by simp
+next
+  case (evtco_return vs env sfs)
+  then show ?case by simp
+next
+  case (evtco_jump v env' cd' r' vs env sfs)
+  then show ?case by simp
+qed
 
 lemma [simp]: "\<Sigma>\<^sub>b \<leadsto>\<^sub>b \<Sigma>\<^sub>b' \<Longrightarrow> orderly_state \<Sigma>\<^sub>b \<Longrightarrow> orderly_state \<Sigma>\<^sub>b'"
 proof (induction \<Sigma>\<^sub>b \<Sigma>\<^sub>b' rule: evalb.induct)
   case (evb_lookup cd pc x env v vs sfs)
-  thus ?case by (cases pc) simp_all
+  thus ?case by (cases pc, cases cd) simp_all
 next
   case (evb_pushcon cd pc k vs env sfs)
-  thus ?case by (cases pc) simp_all
+  thus ?case by (cases pc, cases cd) simp_all
 next
   case (evb_pushlam cd pc pc' vs env sfs)
-  thus ?case by (cases pc) simp_all
+  thus ?case by simp
 next
   case (evb_apply cd pc v env' pc' vs env sfs)
-  thus ?case by (cases pc) simp_all
+  thus ?case by (cases pc', simp, cases pc, cases cd) simp_all
+next
+  case (evb_jump cd pc v env' pc' vs env sfs)
+  thus ?case by (cases pc') simp_all
 qed simp_all
 
 lemma [simp]: "iter (\<leadsto>\<^sub>b) \<Sigma>\<^sub>b \<Sigma>\<^sub>b' \<Longrightarrow> orderly_state \<Sigma>\<^sub>b \<Longrightarrow> orderly_state \<Sigma>\<^sub>b'"
@@ -616,31 +468,28 @@ lemma [simp]: "iter (\<leadsto>\<^sub>t\<^sub>c\<^sub>o) (unflatten_state \<Sigm
   \<exists>\<Sigma>\<^sub>b'. iter (\<leadsto>\<^sub>b) \<Sigma>\<^sub>b \<Sigma>\<^sub>b' \<and> unflatten_state \<Sigma>\<^sub>b' = \<Sigma>\<^sub>t'"
 proof (induction "unflatten_state \<Sigma>\<^sub>b" \<Sigma>\<^sub>t' arbitrary: \<Sigma>\<^sub>b rule: iter.induct)
   case (iter_step \<Sigma>\<^sub>t' \<Sigma>\<^sub>t'')
-  moreover then obtain \<Sigma>\<^sub>b' where S: "iter (\<leadsto>\<^sub>b) \<Sigma>\<^sub>b \<Sigma>\<^sub>b' \<and> unflatten_state \<Sigma>\<^sub>b' = \<Sigma>\<^sub>t'" by fastforcex
-  moreover with iter_step have "orderly_state \<Sigma>\<^sub>b'" by fastforcex
-  ultimately obtain \<Sigma>\<^sub>b'' where "iter (\<leadsto>\<^sub>b) \<Sigma>\<^sub>b' \<Sigma>\<^sub>b'' \<and> unflatten_state \<Sigma>\<^sub>b'' = \<Sigma>\<^sub>t''" by fastforcex
+  moreover then obtain \<Sigma>\<^sub>b' where S: "iter (\<leadsto>\<^sub>b) \<Sigma>\<^sub>b \<Sigma>\<^sub>b' \<and> unflatten_state \<Sigma>\<^sub>b' = \<Sigma>\<^sub>t'" by fastforce
+  moreover with iter_step have "orderly_state \<Sigma>\<^sub>b'" by fastforce
+  ultimately obtain \<Sigma>\<^sub>b'' where "iter (\<leadsto>\<^sub>b) \<Sigma>\<^sub>b' \<Sigma>\<^sub>b'' \<and> unflatten_state \<Sigma>\<^sub>b'' = \<Sigma>\<^sub>t''" by fastforce
   with S show ?case by (metis iter_append)
-qed forcex+
+qed force+
 
-lemma unfl_terminal [simp]: "unflatten_state \<Sigma> = TS [c] [] [] \<Longrightarrow> orderly_state \<Sigma> \<Longrightarrow>
-  \<exists>v cd. \<Sigma> = BS [v] [] [] cd \<and> c = unflatten_closure cd v "
+lemma unfl_terminal [simp]: "unflatten_state \<Sigma> = TCOS [c] [] \<Longrightarrow>
+  \<exists>v cd. \<Sigma> = BS [v] [] cd \<and> c = unflatten_closure cd v"
 proof -
-  assume "unflatten_state \<Sigma> = TS [c] [] []"
-  then obtain vs envs pcs cd where S: "\<Sigma> = BS vs envs pcs cd \<and> [c] = ufcs cd vs \<and> 
-    [] = map (ufcs cd) envs \<and> ufcd cd pcs = []" by (metis unfl_state)
+  assume "unflatten_state \<Sigma> = TCOS [c] []"
+  then obtain vs sfs cd where S: "\<Sigma> = BS vs sfs cd \<and> [c] = ufcs cd vs \<and> [] = ufsfs cd sfs" 
+    by (metis unfl_state)
   moreover then obtain v where "vs = [v] \<and> c = unflatten_closure cd v" by blast
-  moreover from S have "envs = []" by blast
-  moreover assume "orderly_state \<Sigma>"
-  moreover with S have "orderly cd 0 \<and> (\<forall>pc \<in> set pcs. pc \<le> length cd \<and> pc \<noteq> 0)" by simpx
-  ultimately show ?thesis by (metis no_code_poppable)
+  ultimately show ?thesis by simp
 qed
 
-lemma evalb_end [simp]: "iter (\<leadsto>\<^sub>t\<^sub>c\<^sub>o) (unflatten_state \<Sigma>\<^sub>b) (TS [c] []) \<Longrightarrow> orderly_state \<Sigma>\<^sub>b \<Longrightarrow>
+lemma evalb_end [simp]: "iter (\<leadsto>\<^sub>t\<^sub>c\<^sub>o) (unflatten_state \<Sigma>\<^sub>b) (TCOS [c] []) \<Longrightarrow> orderly_state \<Sigma>\<^sub>b \<Longrightarrow>
   \<exists>v. iter (\<leadsto>\<^sub>b) \<Sigma>\<^sub>b (BS [v] [] (code \<Sigma>\<^sub>b)) \<and> c = unflatten_closure (code \<Sigma>\<^sub>b) v"
 proof -
-  assume "iter (\<leadsto>\<^sub>t\<^sub>c\<^sub>o) (unflatten_state \<Sigma>\<^sub>b) (TS [c] [])"
+  assume "iter (\<leadsto>\<^sub>t\<^sub>c\<^sub>o) (unflatten_state \<Sigma>\<^sub>b) (TCOS [c] [])"
   moreover assume O: "orderly_state \<Sigma>\<^sub>b"
-  ultimately obtain \<Sigma>\<^sub>b' where E: "iter (\<leadsto>\<^sub>b) \<Sigma>\<^sub>b \<Sigma>\<^sub>b' \<and> unflatten_state \<Sigma>\<^sub>b' = TS [c] []" 
+  ultimately obtain \<Sigma>\<^sub>b' where E: "iter (\<leadsto>\<^sub>b) \<Sigma>\<^sub>b \<Sigma>\<^sub>b' \<and> unflatten_state \<Sigma>\<^sub>b' = TCOS [c] []" 
     by fastforce
   moreover with O have "orderly_state \<Sigma>\<^sub>b'" by fastforce
   moreover with E obtain v cd where "\<Sigma>\<^sub>b' = BS [v] [] cd \<and> c = unflatten_closure cd v" 
